Docs/ContextualEmbedding/Extrinsic/CEEval.lean
@@ -77,7 +77,7 @@ def eval (typed : CtxHasType ts expr t) (env : Env ts) (fuel : Nat) : Option (Va
   | fuel + 1 =>
       match typed with
       | CtxHasType.CStar => some .star
-      | @CtxHasType.CVar _ _ _ _ _ lookup =>
+      | CtxHasType.CVar lookup =>
           some (env.lookup lookup)
       | @CtxHasType.CLam _ _ body _ bodyTyped =>
           some (.closure env body bodyTyped)
@@ -86,7 +86,7 @@ def eval (typed : CtxHasType ts expr t) (env : Env ts) (fuel : Nat) : Option (Va
           let argValue <- eval argTyped env fuel
           match fnValue with
           | @Val.closure savedTs argTy _ savedEnv body bodyTyped =>
-            let proxy := ProxyTop.PTop (ts := savedTs) (t := argTy)
+            let proxy := ProxyTop.PTop (ts := savedTs :/: argTy)
             eval (bodyTyped proxy) (savedEnv.snoc argValue) fuel
 termination_by fuel
 
